
# 1.
Suppose that $G = D_8 = \langle a, b : a^4 = b^2 = 1, b^{-1} ab = a^{-1} \rangle$.
(a) Let $x$ and $y$ be the following elements of $\mathbb{C}G$:
 $$x = a + 2a^2, \quad y = b + ab - a^2.$$
 Calculate $xy$, $yx$ and $x^2$.
$$xy = (a + 2a^2)(b + ab - a^2)
 = a(b + ab - a^2) + 2a^2(b + ab - a^2)

 = ab + a^2b - aa^2 + 2a^2b + 2a^3b - 2a^4

 = ab + a^2b - a^3 + 2a^2b + 2a^3b - 2

 = ab + 3a^2b + 2a^3b - a^3 - 2$$
 $$yx = (b + ab - a^2)(a + 2a^2) = b(a + 2a^2) + ab(a + 2a^2) - a^2(a + 2a^2) = ba + 2ba^2 + aba + 2aba^2 - a^3 - 2a^4 = a^{-1}b + 2a^{-2}b + a^{-2}b + 2a^{-3}b - a^3 - 2 = a^{-1}b + 3a^{-2}b + 2a^{-3}b - a^3 - 2$$
 
 $$x^2 = (a + 2a^2)^2 = a^2 + 4a^3 + 4a^4 = a^2 + 4a^3 + 4$$

 ---
 
(b) Let $z = b + a^2 b$. Show that $zg = gz$ for all $g \in G$. Deduce that $zr = rz$ for all $r \in \mathbb{C}G$.

 $za = ab + a^{-1}b = az$.
 $zb = 1 + a^2 = bz$.

Since $za = az$ and $zb = bz$, we have shown that $z$ commutes with the generators of $G$.

So, $zg=gz$ for all $g \in G$.


Any element $r \in \mathbb{C}G$ can be written as a linear combination of elements of $G$: $$r = \sum_{g \in G} c_g g, \quad c_g \in \mathbb{C}$$Then,$$zr = z \left( \sum_{g \in G} c_g g \right) = \sum_{g \in G} c_g (zg) = \sum_{g \in G} c_g (gz) = \left( \sum_{g \in G} c_g g \right) z = rz$$ Therefore, $zr = rz$ for all $r \in \mathbb{C}G$.


==$\boxed{zg = gz \text{ for all } g \in G \implies zr = rz \text{ for all } r \in \mathbb{C}G}$

---

# 2.
Work out matrices for the regular representation of $C_2 \times C_2$ over $F$.

$\mathcal{B} = \{e, a, b, ab\}$

Now, $[e]_{\mathcal{B}} = \begin{bmatrix} 1 & 0 & 0 & 0 \\ 0 & 1 & 0 & 0 \\ 0 & 0 & 1 & 0 \\ 0 & 0 & 0 & 1 \end{bmatrix} = I_4$;  $[a]_{\mathcal{B}} = \begin{bmatrix} 0 & 1 & 0 & 0 \\ 1 & 0 & 0 & 0 \\ 0 & 0 & 0 & 1 \\ 0 & 0 & 1 & 0 \end{bmatrix}$;


$[b]_{\mathcal{B}} = \begin{bmatrix} 0 & 0 & 1 & 0 \\ 0 & 0 & 0 & 1 \\ 1 & 0 & 0 & 0 \\ 0 & 1 & 0 & 0 \end{bmatrix}$ ; $[ab]_{\mathcal{B}} = \begin{bmatrix}0 & 0 & 0 & 1 \\ 0 & 0 & 1 & 0 \\ 0 & 1 & 0 & 0 \\ 1 & 0 & 0 & 0 \end{bmatrix}$



---


# 3.
Let $G = C_2$. For $r$ and $s$ in $\mathbb{C}G$, does $rs = 0$ imply that $r = 0$ or $s = 0$?

Soln.
 Let $G = C_2 = {1, g}$ with $g^2 = 1$. Then any $r, s \in \mathbb{C}G$ can be written as:

$$
r = r_1 \cdot 1 + r_2 \cdot g, \quad s = s_1 \cdot 1 + s_2 \cdot g
$$

where $r_1, r_2, s_1, s_2 \in \mathbb{C}$. Multiply:

$$
rs = (r_1 + r_2g)(s_1 + s_2g) = r_1s_1 + r_1s_2g + r_2s_1g + r_2s_2g^2
$$

$$
= r_1s_1 + r_2s_2 + (r_1s_2 + r_2s_1)g
$$

So

$$
rs = (r_1s_1 + r_2s_2) \cdot 1 + (r_1s_2 + r_2s_1) \cdot g
$$

Suppose $rs = 0$. Then:

$$
r_1s_1 + r_2s_2 = 0, \quad r_1s_2 + r_2s_1 = 0
$$

This system has nontrivial solutions. For example:

$$
r = 1 + g, \quad s = 1 - g \Rightarrow rs = (1 + g)(1 - g) = 1 - g^2 = 0
$$

but $r, s \ne 0$. Hence, $\mathbb{C}G$ is **NOT** a domain.

$$
\boxed{\mathbb{C}C_2 \text{ is not a domain; } rs = 0 \nRightarrow r = 0 \text{ or } s = 0}
$$



---

# 4.
 Assume that $G$ is a finite group, say $G = \{g_1, \dots, g_n\}$, and write $c$ for the element $\sum_{i=1}^n g_i$ of $\mathbb{C}G$.
**(a) Prove that $ch = hc = c$ for all $h \in G$.**
Soln.
 Let $G = {g_1, \dots, g_n}$ and define $c = \sum_{i=1}^n g_i \in \mathbb{C}G$. Take any $h \in G$.

Then:

$$
ch = \left(\sum_{i=1}^n g_i\right) h = \sum_{i=1}^n g_i h
$$

Since $h \in G$, the map $g_i \mapsto g_i h$ is a permutation of $G$, so ${g_1 h, \dots, g_n h} = {g_1, \dots, g_n}$. Hence:

$$
ch = \sum_{i=1}^n g_i = c
$$

Similarly:

$$
hc = h \left( \sum_{i=1}^n g_i \right) = \sum_{i=1}^n h g_i
$$

and ${h g_i}$ is again a permutation of $G$, so:

$$
hc = \sum_{i=1}^n g_i = c
$$

Thus:

$$
\boxed{ch = hc = c \quad \text{for all } h \in G}
$$

(b) Deduce that $c^2 = |G|c$.

Soln.
$$
c = \sum_{g \in G} g, \quad \text{so} \quad c^2 = \left( \sum_{g \in G} g \right) \left( \sum_{h \in G} h \right) = \sum_{g, h \in G} gh
$$

Since the product $gh$ ranges over all elements of $G$, and each element appears exactly $|G|$ times (once for each $g$), we get:

$$
c^2 = |G| \sum_{x \in G} x = |G|c
$$

---

(c) Let $\vartheta: \mathbb{C}G \to \mathbb{C}G$ be the linear transformation sending $v$ to $vc$ for all $v$ in $\mathbb{C}G$. What is the matrix $[\vartheta]_{\mathcal{B}}$, where $\mathcal{B}$ is the basis $g_1, \dots, g_n$ of $\mathbb{C}G$?

Soln.
 Since $\vartheta(v) = vc$ and $c = \sum_{j=1}^n g_j$, 

$$\vartheta(g_i) = g_i c = \sum_{j=1}^n g_i g_j$$As $g_i g_j$ runs over all elements of $G$, we get:$$\vartheta(g_i) = \sum_{k=1}^n g_k = c \quad \text{for all } i$$So every basis vector maps to $c = \sum_{k=1}^n g_k$, meaning the matrix $[\vartheta]_{\mathcal{B}}$ has all columns equal to the column vector corresponding to $c$ in the basis $\mathcal{B}$. If we represent $c$ in the basis $\mathcal{B} = \{g_1, \dots, g_n\}$, the coordinates are all $1$. Therefore, the matrix $[\vartheta]_{\mathcal{B}}$ has all columns equal to the column vector of all $1$s:$$[\vartheta]_{\mathcal{B}} = \begin{bmatrix}
1 & 1 & \cdots & 1 \\
1 & 1 & \cdots & 1 \\
\vdots & \vdots & \ddots & \vdots \\
1 & 1 & \cdots & 1
\end{bmatrix} \in M_{n \times n}(\mathbb{C})$$


---

# 5.
If $V$ is an $FG$-module, prove from the definition that
$$0r = 0 \quad \text{for all } r \in FG,$$   $$v0 = 0 \quad \text{for all } v \in V,$$    where the symbol $0$ is used for the zero elements of $V$ and $FG$.

Proof.

 Let $r \in FG$ and $v \in V$. Write $r = \sum_{g \in G} \lambda_g g$.

Since $0 \in V$, by $FG$-module structure:
$$0 \cdot r = 0 \cdot \left( \sum_{g \in G} \lambda_g g \right) = \sum_{g \in G} \lambda_g (0 \cdot g) = \sum_{g \in G} \lambda_g 0 = 0$$Now consider $v \cdot 0$, where $0$ is the zero element of $FG$. We can write $0 = \sum_{g \in G} 0_F g$, where $0_F$ is the zero scalar in $F$. Then:$$v \cdot 0 = v \cdot \left( \sum_{g \in G} 0_F g \right) = \sum_{g \in G} 0_F (v \cdot g) = \sum_{g \in G} 0 = 0$$

---


Show that for every finite group $G$, with $|G| > 1$, there exists an $FG$-module $V$ and elements $v \in V$, $r \in FG$ such that $vr = 0$, but neither $v$ nor $r$ is $0$.

Let $G = \{g_1, \dots, g_n\}$ with $n > 1$, and let $V = FG$ (the regular module). Take:
$$v = g_1 - g_2 \in V \quad (\text{clearly } v \ne 0),$$
$$r = \sum_{i=1}^n g_i \in FG \quad (\text{again } r \ne 0).$$


$$v \cdot r = (g_1 - g_2) \cdot \left( \sum_{i=1}^n g_i \right) = \sum_{i=1}^n g_1 g_i - \sum_{i=1}^n g_2 g_{i}$$

Since $\{g_1 g_i\}_{i=1}^n$ is just a permutation of $G$, and likewise $\{g_2 g_i\}_{i=1}^n$ is another permutation of $G$, we have:
$$\sum_{i=1}^n g_1 g_i = \sum_{h \in G} h \quad \text{and} \quad \sum_{i=1}^n g_2 g_i = \sum_{h \in G} h$$Therefore,$$v \cdot r = \sum_{h \in G} h - \sum_{h \in G} h = 0.$$
Yet $v \ne 0$ and $r \ne 0$,

 so $\boxed{FG \text{ is never a domain}}$.
 
 
# ==we can always construct **nonzero zero divisors** in $FG$==

 ---
 
# 6.
Suppose that $G = D_6 = \langle a, b : a^3 = b^2 = 1, b^{-1} ab = a^{-1} \rangle$, and let $\omega = e^{2\pi i/3}$. Prove that the 2-dimensional subspace $W$ of $\mathbb{C}G$, defined by
$$W = \operatorname{sp}(1 + \omega^2 a + \omega a^2, b + \omega^2 ab + \omega a^2 b),$$
is an irreducible $\mathbb{C}G$-submodule of the regular $\mathbb{C}G$-module.


Let's see how $a$ and $b$ act on the basis of $W = \operatorname{sp}(v_1, v_2)$ where:
$$v_1 = 1 + \omega^2 a + \omega a^2$$
$$v_2 = b + \omega^2 ab + \omega a^2b$$

**Action of $a$**

$$v_1 a = \omega v_1, \quad v_2 a = \omega v_2$$
$$\Rightarrow [a]_W = \begin{pmatrix} \omega & 0 \\ 0 & \omega \end{pmatrix}$$

**Action of $b$**
 $$v_1 b = v_2, \quad v_2 b = v_1$$$$[b]_W = \begin{pmatrix} 0 & 1 \\ 1 & 0 \end{pmatrix}$$


$[a]_W$ is diagonal with eigenvalue $\omega$, so every nonzero vector is an eigenvector of $a$.
$[b]_W$ has no eigenvectors over $\mathbb{C}$ unless $1 = -1$, which it isn’t—its minimal polynomial is $x^2 - 1 = (x - 1)(x + 1)$ but it swaps $v_1 \leftrightarrow v_2$.


So the only subspaces preserved by both are $\{0\}$ and $W$ itself. Hence, $W$ is irreducible.