
# 1.
Let $V$ be a finite-dimensional vector space and let $W_1$ be any subspace of $V$. Prove that there is a subspace $W_2$ of $V$ such that $V = W_1 \oplus W_2$.

Let $W_1$ be a subspace of $V$. Define a linear map $T: V \to W_1$ by projecting each vector onto $W_1$ along some complementary direction. Since $T$ is surjective, by the rankâ€“nullity theorem, $\ker T$ is a subspace $W_2$ such that $V = W_1 \oplus W_2$.

That is, every $v \in V$ can be uniquely written as $v = w_1 + w_2$ with $w_1 \in W_1$, $w_2 \in \ker T$, so $W_2 := \ker T$ gives the desired direct sum.

---
# 2.

Let $V$ be a finite-dimensional vector space and let $W_1, \dots, W_k$ be subspaces of $V$ such that
$V = W_1 + \dots + W_k \quad \text{and} \quad \dim V = \dim W_1 + \dots + \dim W_k.$

Prove that $V = W_1 \oplus \dots \oplus W_k$.

Define linear maps $T_i : W_i \to V$ as the inclusion maps. Each $T_i$ is injective, and the sum $T = T_1 + \dots + T_k : W_1 \oplus \dots \oplus W_k \to V$ is a linear map defined by $T(w_1, \dots, w_k) = w_1 + \dots + w_k$.

Since $V = W_1 + \dots + W_k$, $T$ is surjective. And since $\dim(W_1 \oplus \dots \oplus W_k) = \dim W_1 + \dots + \dim W_k = \dim V$, $T$ is also injective. So $T$ is an isomorphism, meaning $V = W_1 \oplus \dots \oplus W_k$.

Define surjections $\pi_i: V \to W_i$ such that $\pi_i|_{W_i} = \text{id}$ and $\pi_i|_{W_j} = 0$ for $j \ne i$. If $V = W_1 + \dots + W_k$ and the dimension sum matches, then the identity map on $V$ is $\pi_1 + \dots + \pi_k$. Since **the kernel intersection is trivial**, this gives $V = W_1 \oplus \dots \oplus W_k$.

---
# 3.
Find a projection $E$ which projects $\mathbb{R}^2$ onto the subspace spanned by $(1, -1)$ along the subspace spanned by $(1, 2)$.


Let $u = (1, -1)$ and $v = (1, 2)$. For a projection onto $\operatorname{span}\{u\}$ along $\operatorname{span}\{v\}$, we write the projection formula:
$E = \frac{u v^\top}{u^\top v}$
Compute $u^\top v = (1)(1) + (-1)(2) = 1 - 2 = -1$ and $u v^\top = \begin{bmatrix} 1 \\ -1 \end{bmatrix} \begin{bmatrix} 1 & 2 \end{bmatrix} = \begin{bmatrix} 1 & 2 \\ -1 & -2 \end{bmatrix}$.
So:
$E = -\begin{bmatrix} 1 & 2 \\ -1 & -2 \end{bmatrix} = \begin{bmatrix} -1 & -2 \\ 1 & 2 \end{bmatrix}$
This is the projection onto $\operatorname{span}(1, -1)$ along $\operatorname{span}(1, 2)$.

---
# 4.
If $E_1$ and $E_2$ are projections onto independent subspaces, then $E_1 + E_2$ is a projection. True or false?

True.

Let $E_1$ and $E_2$ be projections onto subspaces $V_1$ and $V_2$, respectively, with $V_1 \cap V_2 = \{0\}$. Then $E_1 + E_2$ is a projection onto $V_1 + V_2$ along $\ker(E_1) \cap \ker(E_2)$.
To confirm it's a projection, compute:
$(E_1 + E_2)^2 = E_1^2 + E_1E_2 + E_2E_1 + E_2^2.$

Since $E_i^2 = E_i$ and $E_1E_2 = E_2E_1 = 0$ (follows from independence and action on disjoint subspaces), we get:
$(E_1 + E_2)^2 = E_1 + E_2.$
So $E_1 + E_2$ is idempotent $\Rightarrow$ a projection.

---
# 5.
If $E$ is a projection and $f$ is a polynomial, then $f(E) = aI + bE$. What are $a$ and $b$ in terms of the coefficients of $f$?

$ Let $f(x)=a_0+a_1x+...+a_nx^n,$ where $a_i\in F$. 

Now, $f(E)=a_0I+a_1E+...+a_nE^n$. But, the projection map being idempotent by definition, $E=E^2=...=E^n$. Hence, we end up with $f(E)=a_0I+(a_1+...+a_n)E$.

 Thereby, $a=a_0$, and $b=a_1+...+a_n$.
 
 ---

# 6.
True or false? If a diagonalizable operator has only the characteristic values 0 and 1, it is a projection.

True. A diagonalizable operator with characteristic values $0$ and $1$ is similar to a diagonal matrix with only $0$ and $1$ on the diagonal. Then $T^2$ is similar to that same diagonal matrix squared, which still has only $0$ and $1$ on the diagonal. Hence $T^2 = T$.
So $T$ is idempotent $\Rightarrow$ a projection.

---

# 7.

Prove that if $E$ is the projection on $R$ along $N$, then $(I - E)$ is the projection on $N$ along $R$.

We are given that $E$ is the projection onto $R$ along $N$, so:

$\operatorname{Im}(E) = R$
$\ker(E) = N$
Then consider $I - E$. For any $v \in V$, write $v = r + n$ with $r \in R$, $n \in N$, uniquely. Then
$E(v) = r \quad \Rightarrow \quad (I - E)(v) = v - r = n.$
So $(I - E)(v) = n \in N$, and since $n$ was arbitrary, $\operatorname{Im}(I - E) = N$. Also, $(I - E)(v) = 0$ means $v = E(v) \in R$, so $\ker(I - E) = R$.
Thus, $I - E$ is the projection onto $N$ along $R$.

---
# 8.
Let $E_1, \dots, E_k$ be linear operators on the space $V$ such that $E_1 + \dots + E_k = I$.

(a) Prove that if $E_i E_j = 0$ for $i \ne j$, then $E_i^2 = E_i$ for each $i$.

Let $i$ be fixed. Multiply both sides of $E_1 + \dots + E_k = I$ on the left by $E_i$:
$E_i(E_1 + \dots + E_k) = E_i.$
Since $E_i E_j = 0$ for $i \ne j$, all terms vanish except $E_i E_i$:
$E_i^2 = E_i.$
So each $E_i$ is idempotent.

(b) In the case $k = 2$, prove the converse of (a). That is, if $E_1 + E_2 = I$ and $E_1^2 = E_1$, $E_2^2 = E_2$, then $E_1 E_2 = 0$.

We have $E_2 = I - E_1$.

$E_1 E_2 = E_1(I - E_1) = E_1 - E_1^2 = E_1 - E_1 = 0.$
Similarly, $E_2 E_1 = (I - E_1)E_1 = E_1 - E_1^2 = 0.$

So $E_1 E_2 = E_2 E_1 = 0$.

---

# 9.
Let $V$ be a real vector space and $E$ an idempotent linear operator on $V$, i.e., a projection. Prove that $(I + E)$ is invertible. Find $(I + E)^{-1}$.


**Step 1: Show $\ker(I + E) = \{0\}$**
Suppose $(I + E)v = 0$
$\Rightarrow v = -Ev$
Apply $E$ to both sides:
$Ev = -E^2v = -Ev \Rightarrow 2Ev = 0 \Rightarrow Ev = 0$
Then $v = -Ev = 0$
So $\ker(I + E) = \{0\} \Rightarrow I + E$ is injective. Since $V$ is finite-dimensional, injectivity implies invertibility.

**Step 2: Find inverse**
Try $A = I - \tfrac{1}{2}E$:
$(I + E)(I - \tfrac{1}{2}E) = I - \tfrac{1}{2}E + E - \tfrac{1}{2}E^2 = I.$
Hence,
$(I + E)^{-1} = I - \tfrac{1}{2}E.$

---
# 10.
Let $\mathbb{F}$ be a subfield of the complex numbers (or, a field of characteristic zero). Let $V$ be a finite-dimensional vector space over $\mathbb{F}$. Suppose that $E_1, \dots, E_k$ are projections of $V$ and that $E_1 + \dots + E_k = I$. Prove that $E_i E_j = 0$ for $i \ne j$ (Hint: Use the trace function and ask yourself what the trace of a projection is.)

If $E$ is a projection, then $V = R \oplus N$, where $R = \operatorname{im} E$ and $N = \ker E$. Take a basis $\{\alpha_1, \dots, \alpha_r\}$ of $R$ and extend it with $\{\alpha_{r+1}, \dots, \alpha_n\}$ to a basis of $V$. Then, the matrix of $E$ in this basis is
$$\begin{bmatrix} I_r & 0 \\ 0 & 0 \end{bmatrix},$$
so $\operatorname{tr}(E) = \dim \operatorname{im} E$.

Now note that
$$E_1^2 + E_1E_2 + \dots + E_1E_k = E_1 \Rightarrow E_1^2 - E_1 + \sum_{j \ne 1} E_1E_j = 0.$$
Apply the trace:
$\operatorname{tr}(E_1^2 - E_1) + \sum_{j \ne 1} \operatorname{tr}(E_1E_j) = 0.$
But $E_1^2 = E_1$, so first term is 0. Hence,
$\sum_{j \ne 1} \operatorname{tr}(E_1E_j) = 0.$
Each $\operatorname{tr}(E_1E_j) \ge 0$ since it's the trace of a positive semidefinite operator, so each must be zero. That is,
$\operatorname{tr}(E_iE_j) = 0 \Rightarrow E_iE_j = 0 \quad \text{for } i \ne j.$
This holds symmetrically for all $i, j$.


in short dimension can't be negative

---
# 11.
Let $V$ be a vector space, let $W_1, \dots, W_k$ be subspaces of $V$, and let $$V_{j} = W_1 \oplus \dots \oplus W_{j-1} \oplus W_{j+1} + \dots + W_k.$$

Suppose that $V = W_1 \oplus \dots \oplus W_k$. Prove that the dual space $V^*$ has the direct-sum decomposition $V^* = V_1^0 \oplus \dots \oplus V_k^0$.

Let $f \in V^*$. Since $V = W_1 \oplus \dots \oplus W_k$, every $v \in V$ can be written uniquely as $v = w_1 + \dots + w_k$ with $w_i \in W_i$. Define $f_i(v) = f(w_i)$. Then $f_i$ is linear and vanishes on $V_i = W_1 \oplus \dots \oplus W_{i-1} \oplus W_{i+1} \oplus \dots \oplus W_k$, so $f_i \in V_i^0$. Hence $f = f_1 + \dots + f_k$ with $f_i \in V_i^0$, and $V^* = V_1^0 + \dots + V_k^0$.

To prove the sum is direct, suppose $f \in V_i^0 \cap \sum_{j \ne i} V_j^0$. Then $f = \sum_{j \ne i} f_j$ with $f_j \in V_j^0$. For any $w_i \in W_i$, $f(w_i) = 0$ since $f \in V_i^0$, and also $f_j(w_i) = 0$ for $j \ne i$ since $w_i \in W_i \subset V_j$ for $j \ne i$, so $f(w_i) = \sum_{j \ne i} f_j(w_i) = 0$. Thus $f = 0$, and $V_i^0 \cap \sum_{j \ne i} V_j^0 = \{0\}$. Therefore, $V^* = V_1^0 \oplus \dots \oplus V_k^0$.

---