
# 1.1. 
The identity function $1_X$ on a set $X$ is a permutation, and we usually denote it by $1$. Prove that $1 \circ \sigma = \sigma \circ 1 = \sigma$ for every permutation $\sigma \in S_X$.

Proof.
 trivial exercise to prove identity permutation commutes, work out the algebra, and its done

 *notice that we haven't talked about the group yet, so in general we cant leverage it to the group setting yet* 


---
# 1.2.
 For each $\sigma \in S_X$, prove that there is $\rho \in S_X$ with $\sigma \rho = 1 = \rho \sigma$. (Hint. Let $\rho$ be the inverse function of the bijection $\sigma$).
 
 Proof.
  for any $\alpha \in S_X$ we have a $\beta$ such that they produce 1 on composition
  
  again easy to see that we can always undo a permutation, writing down the algebra in a matter of notation

---

# 1.3.
 For all $\sigma, \rho, \gamma \in S_X$, prove that $\sigma(\rho\gamma) = (\sigma\rho)\gamma$. Indeed, if $X, Y, Z, W$ are sets and $f: X \to Y$, $g: Y \to Z$, and $h: Z \to W$ are functions, then $h \circ (g \circ f) = (h \circ g) \circ f$. (Hint: Recall that two functions $f, g: A \to B$ are equal if and only if, for all $a \in A$, one has $f(a) = g(a)$.)
 
 Proof.
  $$
  ((\sigma \tau) \gamma)(y) = (\sigma \tau)(\gamma(y)) = \sigma (\tau (\gamma(y))).
 $$

$$
  (\sigma (\tau \gamma))(y) = \sigma ((\tau \gamma)(y)) = \sigma (\tau (\gamma(y))).
$$
