
Define a map $\varphi: S \to T$ by
$$\varphi(Hx) = x^{-1}H.$$This is well-defined: if $Hx = Hy$, then $x = hy$ for some $h \in H$, so
$$x^{-1} = y^{-1} h^{-1} \Rightarrow x^{-1}H = y^{-1}H,$$so $\varphi(Hx) = \varphi(Hy)$.
It is injective: if $\varphi(Hx) = \varphi(Hy)$, then $x^{-1}H = y^{-1}H \Rightarrow Hx = Hy$.
It is surjective: for any left coset $aH \in T$, $a^{-1} \in G$ so $H a^{-1} \in S$, and $\varphi(H a^{-1}) = a H$.
Thus, $\varphi$ is a bijection from right cosets to left cosets.

----
Assume:

If $aH = bH$, then $Ha = Hb$.

Take any $a \in G$. Let $b = e$ (identity), so $aH = eH = H$. Then by assumption,

$$Ha = He = H \Rightarrow Ha = H.$$So we have both:

$$aH = H \quad \text{and} \quad Ha = H.$$From $aH = H$, we get $a \in H$.

  

From $Ha = H$, we get $a \in H$ again.

Now take any $h \in H$. We want to show $a h a^{-1} \in H$.

But $a h a^{-1} = a h (a^{-1})$ is a product of elements of $H$ (since $a, h, a^{-1} \in H$), so it lies in $H$.

Hence, $a H a^{-1} \subseteq H$. Similarly, $a^{-1} H a \subseteq H$, so equality holds:

$$a H a^{-1} = H.$$Therefore, $a H a^{-1} = H$ for all $a \in G$; i.e., $H$ is normal in $G$.

---
